CellularAutomatas/proofs/is_two_stage_of_rt_closed_and_prefix_stable.lean
@@ -13,24 +13,11 @@ import Mathlib.Tactic.Linarith
 import Mathlib.Logic.Function.Iterate
 import Mathlib.Data.List.Basic
 import CellularAutomatas.defs
-import CellularAutomatas.proofs.cart_transducers
+import CellularAutomatas.proofs.composition
+import CellularAutomatas.proofs.basic
 import CellularAutomatas.proofs.finite_state_transducers
 
 namespace CellularAutomatas
-
---def extend_word_to k: Word α → Word (Option α)
-/-
-def Lk L k := sorry
-
-
-lemma X (Ls1 Ls2: Set (Language α))
-  (h1: P Ls1) (h2: P Ls2)
-  (h: ∀ L ∈ ℒ CA_rt, ∃ L2 ∈ Ls2, (∀ w ∈ L, w.length.div k) → w ∈ L2):
-    ∀ α, Ls1 α ⊆ Ls2 α := sorry
-
-Let L ∈ Ls1.
-
--/
 
 
 @[simp]
@@ -39,124 +26,14 @@ lemma adv_empty (adv : Advice α Γ) : adv.f [] = [] := by
   rw [List.length_eq_zero_iff.mp h_len]
 
 
-
 lemma tCellAutomatonWithAdvice.elem_L_iff {O: tCellAutomatonWithAdvice α}:
   w ∈ O.L ↔ (O.adv.annotate w) ∈ O.C.L := by rfl
 
-lemma tCellAutomaton.elem_L_iff {C: tCellAutomaton α}:
-  w ∈ C.L ↔ C.F_pos ((C.comp w (C.t w.length)) 0) := by rfl
 
-@[simp]
-lemma scan_temporal_length {C: LCellAutomaton α} (w : Word α) :
-  (C.scan_temporal_rt w).length = w.length := by
-  unfold LCellAutomaton.scan_temporal_rt LCellAutomaton.scan_temporal
-  simp
-
-
-lemma scan_temporal_in_F_pos {C: tCellAutomaton α} (hC: C ∈ CA_rt α) {w: Word α} (i: Nat) (h: i < (C.scan_temporal_rt w).length ):
-    C.F_pos (C.scan_temporal_rt w)[i] = true ↔ w.take (i+1) ∈ C.L := by
-  rw [scan_temporal_length] at h
-  have h_len : i < w.length := h
-  have h_take_len : (w.take (i+1)).length = i + 1 := by
-    rw [List.length_take]
-    rw [min_eq_left]
-    omega
-  have h_t : C.t (w.take (i+1)).length = i := by
-    simp [CA_rt, t_rt] at hC
-    rw [hC.2]
-    rw [h_take_len]
-    simp
-  dsimp [tCellAutomaton.L, Membership.mem, Set.Mem]
-  rw [h_t]
-  unfold LCellAutomaton.scan_temporal_rt LCellAutomaton.scan_temporal
-  rw [List.getElem_map]
-  simp
-  congr 1
-  apply nextt_congr
-  intro j hj
-  unfold LCellAutomaton.embed_word
-  split_ifs with h1 h2
-  · -- j in range of w and w.take
-    unfold Word.get'
-    simp
-  · -- j in range of w but not w.take
-    unfold Word.range at *
-    simp at *
-    grind
-  · -- j not in range of w but in range of w.take
-    unfold Word.range at *
-    simp at *
-    grind
-  · -- neither
-    rfl
-
-def ProdCA (α: Type) (β: Type) [DecidableEq β] [Fintype β] (f: β → LCellAutomaton α): LCellAutomaton α := {
-  Q := ∀ b: β, (f b).Q
-  δ := fun qL qC qR a => (f a).δ (qL a) (qC a) (qR a)
-  embed := fun a b => (f b).embed a
-  border := fun b => (f b).border
-}
-
-namespace ProdCA
-
-
-variable {β: Type} [Alphabet β]
-variable {f: β → LCellAutomaton α}
-
-lemma comp (f: β → LCellAutomaton α)
-    (w: Word α) (t: ℕ) (i: ℤ):
-    (ProdCA α β f).comp w t i = fun b => (f b).comp w t i := by
-  unfold LCellAutomaton.comp
-  unfold CellAutomaton.nextt
-
-  have nextt_proj (c: Config (ProdCA α β f).Q) (t: ℕ) (i: ℤ) (b: β):
-      (ProdCA α β f).next^[t] c i b = (f b).next^[t] (fun j => c j b) i := by
-    induction t generalizing i c with
-    | zero => rfl
-    | succ t ih =>
-      rw [Function.iterate_succ]
-      rw [Function.iterate_succ]
-      dsimp
-      rw [ih]
-      dsimp [CellAutomaton.next, ProdCA]
-      rfl
-
-  funext b
-  simp [apply_iterated]
-  rw [nextt_proj]
-  apply congr_arg (fun c => (f b).next^[t] c i)
-  funext j
-  unfold LCellAutomaton.embed_word
-  dsimp [ProdCA]
-  split_ifs <;> rfl
-
-
--- zipMany over { x => [a, b, c], y => [1, 2, 3] } should be  [ {x => a, y => 1}, {x => b, y => 2}, {x => c, y => 3} ]
-
-def zipMany {γ: β -> Type v} [∀ b, Inhabited (γ b)] (f: (b: β) → Word (γ b)) : Word ((b: β) -> (γ b)) :=
-  let n := (f default).length
-  (List.range n).map fun i => fun b => (f b).getD i default
-
-lemma zipMany_get? {γ: β -> Type v} [∀ b, Inhabited (γ b)] (f: (b: β) → Word (γ b)) (i: ℕ):
-    (ProdCA.zipMany f)[i]? = if i < (f default).length then some (fun b => (f b).getD i default) else none := by
-  simp [zipMany]
-  grind
-
-lemma scan_temporal (f: β → LCellAutomaton α) (w: Word α):
-    (ProdCA α β f).scan_temporal t p w = zipMany (fun b => (f b).scan_temporal t p w) := by
-  unfold LCellAutomaton.scan_temporal
-  simp [zipMany]
-  intro t ht
-  funext b
-  rw [comp]
-  grind
-
-end ProdCA
+-- Reconstruct a two stage advice from a rt-closed and prefix-stable advice
 
 open Classical
 
-
-attribute [ext] Advice
 
 variable {α: Type} [Alphabet α]
 variable {Γ: Type} [Alphabet Γ]
@@ -164,87 +41,34 @@ variable {Γ: Type} [Alphabet Γ]
 def L_c (adv: Advice α Γ) (c: Γ) : Language α :=
   { w | (adv.f w).getLast? = some c }
 
+
+
+/-
+
+
+
+
+
+* L_c := { w | adv.f(w).getLast? = c }
+* (prefix_mem L_c) is two_stage, because L_c is in L(RT-CA) by rt-closedness of adv
+ h: adv.rt_closed
+* ((⊗ fun c => prefix_mem_two_stage L_c h).map_project first_true_or_default).advice = adv
+-/
+
+--
+
 namespace LcInRt
-
-def DiagonalShiftCA (A : Type) [Alphabet A] : LCellAutomaton A := {
-  Q := Option A
-  δ := fun _ _ r => r
-  embed := some
-  border := none
-}
-
-@[simp]
-lemma DiagonalShiftCA_comp_p0  (w : Word α) :
-  (DiagonalShiftCA α).comp w t 0 = w[t]? := by
-  unfold LCellAutomaton.comp
-
-  have shift_next c : (DiagonalShiftCA α).next c = fun i => c (i + 1) := by
-    funext i
-    simp [CellAutomaton.next, DiagonalShiftCA]
-
-  have shift_nextt k c i: ((DiagonalShiftCA α).nextt c k) i = c (i + k) := by
-    induction k generalizing c with
-    | zero =>
-      simp [CellAutomaton.nextt, apply_iterated]
-    | succ k ih =>
-      rw [CellAutomaton.nextt, apply_iterated]
-      simp only [Nat.iterate]
-      rw [shift_next]
-      rw [← apply_iterated]
-      rw [← CellAutomaton.nextt]
-      rw [ih]
-      simp
-      ring_nf
-
-  rw [shift_nextt]
-  unfold LCellAutomaton.embed_word
-  dsimp [DiagonalShiftCA]
-  unfold Word.get'
-  unfold Word.range
-  grind
-
-lemma DiagonalShiftCA_scan_temporal {Q : Type} [Alphabet Q] (w : Word Q) :
-  (DiagonalShiftCA Q).scan_temporal_rt w = w.map some := by
-  unfold LCellAutomaton.scan_temporal_rt LCellAutomaton.scan_temporal
-  apply List.ext_getElem
-  · simp
-  · intro i h_i h_len
-    simp [←getElem?_pos]
 
 
 def AdvCALc (c : Γ) : tCellAutomaton (α × Γ) := {
-  toLCellAutomaton := DiagonalShiftCA (α × Γ)
+  toCellAutomaton := (ca_id_word (α × Γ)).map_project (fun (_, g) => g == c)
   t := fun n => n - 1
   p := fun _ => 0
-  F_pos := fun q => match q with
-    | some (_, g) => g == c
-    | none => false
 }
 
 lemma myCA_in_rt (c : Γ) : AdvCALc c ∈ CA_rt (α × Γ) := by
-  simp [CA_rt, t_rt, AdvCALc, tCellAutomatons, CA]
+  simp [CA_rt, t_rt, AdvCALc, tCellAutomata, CA]
 
-lemma scan_temporal_get_last {C: tCellAutomaton α} (w : Word α):
-  (C.scan_temporal_rt w).getLast? = if w = [] then none else ((C.comp w (w.length - 1)) 0) := by
-  cases h_w : w.length with
-  | zero =>
-    simp [LCellAutomaton.scan_temporal_rt, LCellAutomaton.scan_temporal]
-    have h_nil : w = [] := List.length_eq_zero_iff.mp h_w
-    subst h_nil
-    unfold LCellAutomaton.comp
-    unfold LCellAutomaton.embed_word
-    simp
-  | succ n =>
-    have h_len_pos : w.length > 0 := by rw [h_w]; simp
-    have h_scan_len : (C.scan_temporal_rt w).length = w.length := scan_temporal_length w
-    have h_scan_pos : (C.scan_temporal_rt w).length > 0 := by rw [h_scan_len]; exact h_len_pos
-
-    rw [List.getLast?_eq_some_getLast (List.ne_nil_of_length_pos h_scan_pos)]
-    simp
-    rw [List.getLast_eq_getElem]
-    unfold LCellAutomaton.scan_temporal_rt LCellAutomaton.scan_temporal
-    simp
-    grind
 
 
 def O (adv : Advice α Γ) (c : Γ) : tCellAutomatonWithAdvice α := ⟨Γ, adv, AdvCALc c⟩
@@ -257,7 +81,7 @@ lemma O_L_eq_L_c (adv : Advice α Γ) (c : Γ) : (O adv c).L = L_c adv c := by
   have h_len : w_ann.length = w.length := by
     simp [w_ann, Advice.annotate, zip_words, adv.len]
 
-  change (AdvCALc c).F_pos ((AdvCALc c).comp w_ann ((AdvCALc c).t w_ann.length) 0) ↔ (adv.f w).getLast? = some c
+  change ((AdvCALc c).comp w_ann ((AdvCALc c).t w_ann.length) 0) ↔ (adv.f w).getLast? = some c
   dsimp [AdvCALc]
   rw [DiagonalShiftCA_comp_p0]
 
@@ -334,16 +158,14 @@ namespace PrefixStableProof
 
   variable (adv: Advice α Γ) (h1: adv.rt_closed)
 
-  noncomputable abbrev M_prod := ProdCA α Γ (fun c => (CALc adv h1 c).toLCellAutomaton)
+  noncomputable abbrev M_prod := ProdCA (fun c => (CALc adv h1 c).toCellAutomaton)
 
-  noncomputable def t_map (q: (M_prod adv h1).Q) : Γ :=
-    let valid_c := Finset.univ.filter (fun c => (CALc adv h1 c).F_pos (q c))
+  noncomputable def first_true_or_default (q: Γ → Bool) : Γ :=
+    let valid_c := Finset.univ.filter (fun c => q c)
     valid_c.toList.head?.getD default
 
-
-
   noncomputable def ts_adv : TwoStageAdvice α Γ := {
-    C := ⟨ M_prod adv h1, t_map adv h1 ⟩
+    C := (M_prod adv h1).map_project first_true_or_default
     β := Γ
     M := FiniteStateTransducer.M_id Γ
   }
@@ -358,14 +180,11 @@ namespace PrefixStableProof
     unfold ts_adv
     simp
 
-    unfold CArtTransducer.advice
-    simp [LCellAutomaton.scan_temporal_rt]
-    rw [ProdCA.scan_temporal]
-    conv =>
-      pattern LCellAutomaton.scan_temporal _ _ _ _
-      rw [←LCellAutomaton.scan_temporal_rt]
+    rw [ProdCA.trace_rt]
 
     apply List.ext_getElem?
+
+
 
     intro i
     rw [List.getElem?_map]
@@ -375,7 +194,7 @@ namespace PrefixStableProof
     by_cases h_i : i < w.length
     case neg => simp [h_i]
 
-    unfold t_map
+    unfold first_true_or_default
     simp
 
 
