CellularAutomatas/proofs/basic.lean
@@ -1,0 +1,427 @@
+import CellularAutomatas.defs
+import Mathlib.Data.List.Basic
+import Mathlib.Data.Nat.Basic
+import Mathlib.Data.Nat.Find
+import Mathlib.Data.Int.Cast.Basic
+import Mathlib.Data.Fintype.Option
+import Mathlib.Tactic.Ring
+
+namespace CellularAutomatas
+
+
+private lemma list_map_congr {α β} {f g : α → β} {l : List α} (h : ∀ x ∈ l, f x = g x) : l.map f = l.map g := by
+  induction l with
+  | nil => rfl
+  | cons a l ih =>
+  simp only [List.map_cons, List.cons.injEq]
+  constructor
+  · apply h; simp
+  · apply ih; intro x hx; apply h; simp [hx]
+
+
+lemma nextt_congr {α β} (C: CellAutomaton α β) (c1 c2: Config C.Q) (t: ℕ) (i: ℤ):
+    (∀ j, i - t ≤ j ∧ j ≤ i + t → c1 j = c2 j) →
+    (C.nextt c1 t) i = (C.nextt c2 t) i := by
+  induction t generalizing i c1 c2 with
+  | zero =>
+    intro h
+    simp [CellAutomaton.nextt]
+    apply h
+    constructor <;> omega
+  | succ t ih =>
+    intro h
+    simp [CellAutomaton.nextt]
+    -- The goal is now nextt (next c1) t i = nextt (next c2) t i
+    apply ih
+    intro j hj
+    unfold CellAutomaton.next
+    congr 1
+    · apply h
+      constructor <;> omega
+    · apply h
+      constructor <;> omega
+    · apply h
+      constructor <;> omega
+
+lemma LCellAutomaton.scan_temporal_independence_at_0 {β} [Alphabet β] (C: CellAutomaton α？ β) (p s: Word α) (t: ℕ) (ht: t < p.length):
+  (C.nextt ⦋⟬p ++ s⟭⦌ t) 0 = (C.nextt ⦋⟬p⟭⦌ t) 0 := by
+  apply nextt_congr
+  intro j hj
+  simp only [zero_sub, zero_add] at hj
+  delta embed_word word_to_config
+  unfold CellAutomaton.embed_config
+  by_cases h_if : j ≥ 0 ∧ j < ↑(List.length (p ++ s))
+  · have h_if_p : j ≥ 0 ∧ j < ↑(List.length p) := by
+      constructor
+      · exact h_if.1
+      · have : j ≤ t := hj.2
+        have : t < p.length := ht
+        omega
+    grind
+  · have h_if_p : ¬(j ≥ 0 ∧ j < ↑(List.length p)) := by
+      intro h
+      apply h_if
+      constructor
+      · exact h.1
+      · apply lt_of_lt_of_le h.2
+        simp
+    grind
+
+@[simp]
+theorem LCellAutomaton.scan_temporal_independence {β} [Alphabet β] (C: CellAutomaton α？ β) (p s: Word α):
+  (C.trace_rt (p ++ s)).take p.length = C.trace_rt p := by
+  unfold CellAutomaton.trace_rt
+  rw [← List.map_take, List.take_range, min_eq_left (by simp)]
+  apply list_map_congr
+  intro t ht
+  rw [List.mem_range] at ht
+  unfold CellAutomaton.trace CellAutomaton.comp CellAutomaton.project_config
+  simp only [Function.comp_apply]
+  congr 1
+  apply LCellAutomaton.scan_temporal_independence_at_0
+  exact ht
+
+@[simp]
+theorem CArtTransducer.scan_temporal_independence [Alphabet α] [Alphabet Γ] (C: CArtTransducer α Γ) (p s: Word α):
+  (C.advice.f (p ++ s)).take p.length = C.advice.f p := by
+  unfold CArtTransducer.advice
+  simp
+
+
+
+open CellAutomaton
+
+@[simp]
+lemma trace_of_map_project {α β γ: Type} {C: CellAutomaton α？ β} (f: β → γ) (w: Word α):
+      (C.map_project f).trace w = f ∘ (C.trace w) := by
+  funext i
+  unfold trace comp project_config
+  simp
+  unfold map_project
+  rfl
+
+@[simp]
+lemma trace_rt_of_map_project {α β γ: Type} {C: CellAutomaton α？ β} (f: β → γ) (w: Word α):
+      (C.map_project f).trace_rt w = (C.trace_rt w).map f := by
+  unfold trace_rt
+  apply List.ext_getElem (by simp)
+  intro i h1 h2
+  simp
+
+@[simp]
+lemma trace_rt_length {α β: Type} {C: CellAutomaton α？ β} {w: Word α}:
+  (C.trace_rt w).length = w.length := by simp [trace_rt]
+
+
+
+@[grind =]
+lemma word_to_config_natcast_eq {w: Word α} {t: ℕ} (h: t < w.length): ⟬w⟭ ↑t = some w[t] := by simp [word_to_config, h]
+
+
+
+
+
+
+lemma tCellAutomaton.elem_L_iff {C: tCellAutomaton α}:
+  w ∈ C.L ↔ ((C.comp w (C.t w.length)) (C.p w.length)) := by rfl
+
+
+@[simp]
+lemma CA_rt_t (C: CA_rt α) (n: Nat) :
+  C.val.t n = n - 1 := by
+  unfold CA_rt t_rt at C
+  grind
+
+@[simp]
+lemma CA_rt_p (C: CA_rt α) (n: Nat) :
+  C.val.p n = 0 := by
+  unfold CA_rt CA t_rt at C
+  grind
+
+lemma CA_rt_L_iff {C: CA_rt α}:
+  w ∈ C.val.L ↔ (C.val.comp w (w.length - 1)) 0 = true := by
+  simp [tCellAutomaton.elem_L_iff, CA_rt_t, CA_rt_p]
+
+lemma trace_L {C: CA_rt α} {w: Word α}: C.val.trace w (w.length - 1) = true ↔ w ∈ C.val.L := by
+  simp [CellAutomaton.trace, CA_rt_L_iff]
+
+@[simp]
+lemma trace_rt_neq_empty {C: CellAutomaton (Option α) β} {w: Word α}: (C.trace_rt w) ≠ [] ↔ w ≠ [] := by
+  simp [←List.length_eq_zero_iff]
+
+lemma trace_rt_L {C: CA_rt α} {w: Word α} (h: w ≠ []):
+  (C.val.trace_rt w).getLast (by simp [h]) = true ↔ w ∈ C.val.L := by
+  simp [List.getLast_eq_getElem, CellAutomaton.trace_rt, trace_L]
+
+
+lemma trace_rt_getElem_i_iff {C: CA_rt α} {w: Word α} (i: Nat) (h: i < (C.val.trace_rt w).length ):
+    (C.val.trace_rt w)[i] = true ↔ w.take (i+1) ∈ C.val.L := by
+  sorry
+
+
+
+
+
+
+def config_to_trace {α: Type} (c: Config α): Trace α := fun t => c t
+
+section id
+
+  def ca_id (α : Type) [Alphabet α] : CellAutomaton α α := {
+    Q := α
+    δ := fun _ _ r => r
+    embed := id
+    project := id
+  }
+
+
+  @[simp]
+  lemma ca_id_trace_eq {α : Type} [Alphabet α]:
+    (ca_id α).trace = config_to_trace := by
+    unfold trace
+    funext t
+    conv in comp _ => change nextt _
+
+    have shift_next c : (ca_id α).next c = fun i => c (i + 1) := by
+      funext i
+      simp [CellAutomaton.next, ca_id]
+
+    have shift_nextt k c i: ((ca_id α).nextt c k) i = c (i + k) := by
+      induction k generalizing c i with
+      | zero =>
+        simp
+      | succ k ih =>
+        rw [CellAutomaton.nextt_succ]
+        rw [shift_next]
+        simp
+        rw [ih]
+        grind
+    funext t
+    rw [shift_nextt]
+    conv in embed_config => change id
+    simp [config_to_trace]
+
+
+
+  def ca_id_word (α: Type) [Alphabet α] : CellAutomaton α？ α := (ca_id α？).map_project (·.getD default)
+
+  @[simp]
+  lemma ca_id_scan_temporal [Alphabet α]: (ca_id_word α).trace_rt = id := by
+    funext w
+    rw [id_eq, ca_id_word, trace_rt_of_map_project]
+    apply List.ext_getElem (by simp)
+    intro i h_i h_len
+    unfold trace_rt
+    simp [ca_id_trace_eq]
+    grind [ca_id_trace_eq, config_to_trace]
+
+end id
+
+
+
+
+
+
+
+
+def ProdCA {α P γ: Type} [Alphabet P] (f: P → CellAutomaton α γ): CellAutomaton α (P → γ) := {
+  Q := ∀ b: P, (f b).Q
+  δ := fun qL qC qR a => (f a).δ (qL a) (qC a) (qR a)
+  embed := fun a b => (f b).embed a
+  project := fun q => (fun b => (f b).project (q b))
+}
+
+namespace ProdCA
+
+  variable {α P γ: Type} [Alphabet P]
+  variable {f: P → CellAutomaton α γ}
+
+  lemma comp [Alphabet γ] (f: P → CellAutomaton (Option α) γ)
+      (w: Word α) (t: ℕ) (i: ℤ):
+      (ProdCA f).comp w t i = fun b => (f b).comp w t i := by
+    unfold CellAutomaton.comp CellAutomaton.project_config
+    unfold CellAutomaton.nextt
+
+    have nextt_proj (c: Config (ProdCA f).Q) (t: ℕ) (i: ℤ) (b: P):
+        (ProdCA f).next^[t] c i b = (f b).next^[t] (fun j => c j b) i := by
+      induction t generalizing i c with
+      | zero => rfl
+      | succ t ih =>
+        rw [Function.iterate_succ]
+        rw [Function.iterate_succ]
+        dsimp
+        rw [ih]
+        dsimp [CellAutomaton.next, ProdCA]
+        rfl
+
+    funext b
+    simp
+    conv in (ProdCA f).project =>
+      simp [ProdCA]
+    rw [nextt_proj]
+    congr
+
+
+  -- zipMany over { x => [a, b, c], y => [1, 2, 3] } should be  [ {x => a, y => 1}, {x => b, y => 2}, {x => c, y => 3} ]
+
+  def zipMany {γ: P -> Type v} [∀ b, Inhabited (γ b)] (f: (b: P) → Word (γ b)) : Word ((b: P) -> (γ b)) :=
+    let n := (f default).length
+    (List.range n).map fun i => fun b => (f b).getD i default
+
+  lemma zipMany_get? {γ: P -> Type v} [∀ b, Inhabited (γ b)] (f: (b: P) → Word (γ b)) (i: ℕ):
+      (ProdCA.zipMany f)[i]? = if i < (f default).length then some (fun b => (f b).getD i default) else none := by
+    simp [zipMany]
+    grind
+
+  @[simp]
+  lemma trace_rt [Alphabet γ] (f: P → CellAutomaton (Option α) γ) (w: Word α):
+      (ProdCA f).trace_rt w = zipMany (fun b => (f b).trace_rt w) := by
+    unfold CellAutomaton.trace_rt CellAutomaton.trace
+    simp [zipMany]
+    intro t ht
+    funext b
+    rw [comp]
+    grind
+
+end ProdCA
+
+
+def ca_zip {α β1 β2} [Alphabet α] [Alphabet β1] [Alphabet β2]
+  (C1: CellAutomaton α β1) (C2: CellAutomaton α β2) :
+    CellAutomaton α (β1 × β2) :=
+  (ProdCA
+    (fun
+      | (0: Fin 2) => C1.map_project (fun v => (v, default))
+      | (1: Fin 2) => C2.map_project (fun v => (default, v))
+    )
+  ).map_project (fun v => ((v 0).fst, (v 1).snd))
+
+
+infixr:90 "⨂"  => ca_zip
+
+
+
+@[simp]
+lemma ca_zip_trace_rt {α β1 β2} [Alphabet α] [Alphabet β1] [Alphabet β2]
+    {C1: CellAutomaton α？ β1} {C2: CellAutomaton α？ β2} {w: Word α}:
+    (C1 ⨂ C2).trace_rt w = (C1.trace_rt w) ⨂ (C2.trace_rt w) := by
+  unfold ca_zip
+  simp
+  apply List.ext_getElem?
+  intro i
+  simp [ProdCA.zipMany_get?]
+  by_cases h: i < List.length w
+  · simp [h, zip_words]
+  · simp [h, zip_words]
+
+
+
+
+def word_dvd_k_ext (k: ℕ) (w_len: ℕ) := (w_len - (w_len % w_len)) % w_len
+
+def word_dvd_k (k: ℕ) (w: Word α): Word (Option α) :=
+  w.map (fun a => some a) ++ List.replicate (word_dvd_k_ext k w.length) none
+
+def L_dvd_k (k: ℕ) (L: Language α): Language (Option α) := { word_dvd_k k w | w ∈ L }
+
+theorem L_in_RT_iff_L_dvd_k_in_RT [Alphabet α] (k: ℕ) (L: Language α):
+    L ∈ ℒ (CA_rt α) ↔ (L_dvd_k k L) ∈ ℒ (CA_rt (Option α)) := by
+  sorry
+
+
+
+
+
+
+
+@[simp]
+lemma nextt0 (C: CellAutomaton α β) (c: Config C.Q): C.nextt c 0 = c := by simp [CellAutomaton.nextt]
+
+@[simp]
+lemma nextt1 (C: CellAutomaton α β) (c: Config C.Q): C.nextt c 1 = C.next c := by simp [CellAutomaton.nextt]
+
+/-
+lemma LCellAutomaton.embed_word_eq (C: LCellAutomaton α) {w: Word α} {p: ℤ} (h: p ∈ w.range):
+    C.embed_word w p = C.embed (w.get' p h) := by
+      grind [LCellAutomaton.embed_word, Word.get']
+-/
+
+
+lemma LCellAutomaton.nextt_succ_eq (C: LCellAutomaton α) (c: Config C.Q): C.nextt c (t + 1) = C.next (C.nextt c t) := by
+  simp [CellAutomaton.nextt]
+  sorry
+
+
+/-
+lemma LCellAutomaton.comp_succ_eq (C: LCellAutomaton α): C.comp w (t + 1) = C.next (C.comp w t) := by
+  funext i
+  simp [LCellAutomaton.comp, LCellAutomaton.nextt_succ_eq]
+-/
+
+
+
+
+
+variable [Alphabet α] [Alphabet Γ]
+
+lemma ℒ_CA_rt_iff {α} [Alphabet α] {L: Language α}: L ∈ ℒ (CA_rt α) ↔ ∃ C ∈ CA_rt α, C.L = L := by
+  simp [tCellAutomata, CA_rt, t_rt]
+  unfold ℒ
+  unfold DefinesLanguage.L instDefinesLanguageTCellAutomatonOfAlphabet
+  simp
+  sorry
+
+
+lemma ℒ_oca_def (adv: Advice α Γ) (L: Language α):
+      L ∈ ℒ (CA_rt (α × Γ) + adv) ↔ ∃ C ∈ CA_rt (α × Γ), L = { w | (w ⨂ (adv.f w)) ∈ C.L } := by
+  --simp [ℒ, tCellAutomatonWithAdvice.with_advice, tCellAutomatonWithAdvice.L, Advice.annotate]
+  sorry
+
+lemma ℒ_tCellAutomaton_def (L: Language α):
+        L ∈ ℒ (CA_rt α) ↔ ∃ C ∈ CA_rt α, C.L = L := by
+  --simp [ℒ]
+  sorry
+
+
+
+
+
+
+
+
+
+
+  section
+    lemma embed_word_at_eq {α β: Type} (w: Word α) {C: CellAutomaton α？ β} (p: ℤ):
+        @embed_word α β C w p = C.embed (if h: p ∈ w.range then  (some (w.get' p h)) else none) := by rfl
+
+    @[simp]
+    lemma embed_word_at_eq1 {α β: Type} (w: Word α) {C: CellAutomaton α？ β} (p: ℤ) (h: p ∈ w.range):
+        @embed_word α β C w p = C.embed (some (w.get' p h)) := by simp [embed_word_at_eq, h]
+
+    @[simp]
+    lemma embed_word_at_eq2 {α β: Type} (w: Word α) {C: CellAutomaton α？ β} (p: ℤ) (h: ¬(p ∈ w.range)):
+        @embed_word α β C w p = C.embed none := by simp [embed_word_at_eq, h]
+
+  end
+
+  @[simp]
+  lemma project_config_at {α β: Type} [Alphabet α] [Alphabet β] {C: CellAutomaton α？ β} (p: ℤ) {c: Config C.Q}:
+    C.project_config c p = C.project (c p) := by rfl
+
+  lemma comp_eq_project_nextt {α β: Type} {C: CellAutomaton α？ β} (w: Word α) (t: ℕ):
+      C.comp w t = C.project_config (C.nextt w t) := by rfl
+
+
+
+
+
+
+
+
+@[simp]
+lemma Word.get'_eq {α} (w: Word α) (i: ℕ) (h: i < w.length) (val: α): (w.get'? ↑i).getD val = w[i] := by
+  unfold Word.get'?
+  by_cases h: ↑↑i ∈ w.range
+  simp [h, Word.get']
+  simp_all [Word.range]
