CellularAutomatas/proofs/two_stage_is_rt_closed.lean
@@ -1,0 +1,176 @@
+import Mathlib.Data.Set.Basic
+import Mathlib.Data.Nat.Basic
+import Mathlib.Data.Nat.Find
+import Mathlib.Data.Fintype.Basic
+import Mathlib.Data.Fintype.Pi
+import Mathlib.Data.Fintype.Option
+import Mathlib.Computability.Language
+import Mathlib.Data.Set.Lattice
+import Mathlib.Data.Nat.Lattice
+import Mathlib.Data.Fintype.Prod
+import Mathlib.Tactic.Ring
+import Mathlib.Tactic.Linarith
+import Mathlib.Logic.Function.Iterate
+import Mathlib.Data.List.Basic
+import CellularAutomatas.defs
+import CellularAutomatas.proofs.composition
+import CellularAutomatas.proofs.basic
+import CellularAutomatas.proofs.finite_state_transducers
+import CellularAutomatas.proofs.advice_two_stage_closed_under_composition
+
+namespace CellularAutomatas
+
+variable {α Γ : Type} [Alphabet α] [Alphabet Γ]
+
+open FiniteStateTransducer (M_map M_prod M_projQ M_id)
+open CellAutomaton
+
+
+def prefix_mem (L: Language α) [DecidablePred L] (w: Word α): Word Bool :=
+  (List.range w.length).map (fun i => decide (L (w⟦0..i+1⟧)))
+
+@[simp]
+lemma prefix_mem_len {α} (L: Language α) [DecidablePred L] (w: Word α):
+  (prefix_mem L w).length = w.length := by
+  simp [prefix_mem]
+
+def prefix_mem_adv (L: Language α) [DecidablePred L]: Advice α Bool := { f := prefix_mem L }
+
+def lift {α β} [Alphabet α] [Alphabet β]
+    (f: Word α → Word β) (L: Language α): Language β :=
+  { w: Word β | ∃ v: Word α, f v = w ∧ L v }
+
+
+
+
+
+
+
+
+
+
+variable {α: Type} [Alphabet α]
+variable {Γ: Type} [Alphabet Γ]
+
+def CA_rt_to_TwoStage (C: CA_rt α): TwoStageAdvice α Bool :=
+  {
+    β := Bool
+    C := C.val.toCellAutomaton
+    M := FiniteStateTransducer.M_id Bool
+  }
+
+lemma CA_rt_to_TwoStage_advice_eq (C: CA_rt α) :
+  (CA_rt_to_TwoStage C).advice.f = C.val.trace_rt := by
+  funext w
+  simp [CA_rt_to_TwoStage, TwoStageAdvice.advice]
+
+lemma CA_rt_to_TwoStage_eq (C: CA_rt α):
+  (CA_rt_to_TwoStage C).advice.f = (Advice.prefixes_in_L C.val.L).f := by
+  rw [CA_rt_to_TwoStage_advice_eq]
+  funext w
+  apply List.ext_getElem
+  · simp
+  · intro i h1 h2
+    have (v: Bool) (p: Prop) [Decidable p]: (v = decide p ↔ (v = true ↔ p)) := by grind
+    simp [Advice.prefixes_in_L, this, trace_rt_getElem_i_iff]
+    rfl
+
+
+theorem advice_prefixes_in_L_is_two_stage_advice (C: CA_rt α):
+    (Advice.prefixes_in_L C.val.L).is_two_stage_advice := by
+  use CA_rt_to_TwoStage C
+  have h_eq := CA_rt_to_TwoStage_eq C
+  match (CA_rt_to_TwoStage C).advice, (Advice.prefixes_in_L C.val.L), h_eq with
+  | ⟨f1, l1⟩, ⟨f2, l2⟩, h =>
+    simp at h
+    subst h
+    rfl
+
+
+
+noncomputable def get_ca (L: ℒ (CA_rt α)): CA_rt α := by
+  have := L.prop
+  rw [ℒ_CA_rt_iff] at this
+  exact ⟨ Classical.choose this, by simp [Classical.choose_spec this] ⟩
+
+
+noncomputable def prefix_mem_two_stage (L: ℒ (CA_rt α)): TwoStageAdvice α Bool :=
+  CA_rt_to_TwoStage (get_ca L)
+
+def prefix_mem_two_stage_spec (L: ℒ (CA_rt α)) [DecidablePred L.val]:
+    (prefix_mem_two_stage L).advice.f = prefix_mem L.val := by
+  sorry
+
+lemma advice_eq_iff {α β: Type} (adv1 adv2: Advice α β) (h: adv1.f = adv2.f): adv1 = adv2 := by
+  cases adv1
+  cases adv2
+  simp at h
+  subst h
+  rfl
+
+
+lemma L_rt_iff_prefix_mem_two_stage (L: Language α) [DecidablePred L]:
+    L ∈ ℒ (CA_rt α) ↔ (prefix_mem_adv L).is_two_stage_advice := by
+  constructor
+  · intro h
+    use prefix_mem_two_stage (⟨L, h⟩ : ℒ (CA_rt α))
+    apply advice_eq_iff
+    simp [prefix_mem_adv, prefix_mem_two_stage_spec]
+  · intro h
+    rw [ℒ_CA_rt_iff]
+    sorry
+
+
+-- classical
+
+def ca_to_two_stage (C: CArtTransducer α Γ): TwoStageAdvice α Γ :=
+  {
+    β := Γ
+    C := C
+    M := FiniteStateTransducer.M_id Γ
+  }
+
+
+def zip_two_stage [Alphabet α] [Alphabet β] [Alphabet γ] (a1: TwoStageAdvice α β) (a2: TwoStageAdvice α γ):
+    TwoStageAdvice α (β × γ) :=
+  let ca_new := a1.C ⨂ a2.C
+  let fst_new := a1.M ⨂ a2.M
+  TwoStageAdvice.from_transducers fst_new ca_new
+
+infixl:65 " ⨂ " => zip_two_stage
+
+noncomputable def A (adv: TwoStageAdvice α Γ) (L: Language α): TwoStageAdvice α Bool :=
+  (prefix_mem_two_stage ⟨(lift adv.advice.annotate L), sorry⟩) ⊚ ((ca_to_two_stage (ca_id_word α)) ⨂ adv)
+
+lemma A_spec (adv: TwoStageAdvice α Γ) (L: Language α) [DecidablePred L]:
+    (A adv L).advice = prefix_mem_adv L := by
+  apply advice_eq_iff
+  funext w
+  simp [A, TwoStageAdvice.advice]
+  sorry
+
+lemma rt_closed_iff (adv: Advice α Γ):
+    adv.rt_closed ↔ (∀ L, (lift adv.annotate L) ∈ ℒ (CA_rt (α × Γ)) → L ∈ ℒ (CA_rt α)) := by
+
+  unfold Advice.rt_closed
+  unfold adviceAdd
+  conv in (ℒ (CA_rt (α ⨉ Γ) + adv) ) =>
+    change L ∈ tCellAutomatonWithAdvice.with_advice (CA_rt (α × Γ)) adv
+
+  sorry
+
+
+theorem two_stage_rt_closed (adv: TwoStageAdvice α Γ):
+    adv.advice.rt_closed := by
+  open Classical in -- I'm quite sure this is not needed
+
+  suffices ∀ (L : Language α) (h: lift adv.advice.annotate L ∈ ℒ (CA_rt (α ⨉ Γ))), L ∈ ℒ (CA_rt α) from by
+    simp_all [rt_closed_iff]
+
+  intro L h
+
+  suffices ∃ ts_adv: TwoStageAdvice α Bool, ts_adv.advice = prefix_mem_adv L from by
+    simp_all [L_rt_iff_prefix_mem_two_stage, Advice.is_two_stage_advice]
+
+  use A adv L
+  simp [A_spec adv]
