CellularAutomatas_old/defs.lean
@@ -1,0 +1,482 @@
+import Mathlib.Data.Set.Basic
+import Mathlib.Data.Nat.Basic
+import Mathlib.Data.Nat.Find
+import Mathlib.Data.Fintype.Basic
+import Mathlib.Data.Fintype.Pi
+import Mathlib.Computability.Language
+import Mathlib.Data.Set.Lattice
+import Mathlib.Data.Nat.Lattice
+import Mathlib.Data.Fintype.Prod
+
+namespace CellularAutomatas
+
+section Utilities -- MARK: Utilities
+
+  noncomputable def min_nat (set: Set ℕ) :=
+    let _dec := Classical.dec;
+    if h: ∃ n, n ∈ set
+    then some (Nat.find h)
+    else none
+
+  def apply_iterated (f: α → α) (a: α) (k: ℕ) := Nat.iterate f k a
+
+end Utilities
+
+
+
+section Word -- MARK: Word
+
+  class Alphabet (α: Type) where
+    [dec: DecidableEq α]
+    [fin: Fintype α]
+    [inh: Inhabited α]
+
+  attribute [instance] Alphabet.dec Alphabet.fin Alphabet.inh
+
+  instance (α: Type) [DecidableEq α] [Fintype α] [Inhabited α]: Alphabet α := {}
+
+  instance AlphabetUnit : Alphabet Unit := {}
+  instance AlphabetBool : Alphabet Bool := {}
+  instance ProductAlphabet {α β: Type} [Alphabet α] [Alphabet β] : Alphabet (α × β) := {}
+  instance FunctionAlphabet {α β: Type} [Alphabet α] [Alphabet β] : Alphabet (α → β) := {}
+
+  infix:50 " ⨉ " => Prod
+
+
+  abbrev Word (α: Type u) := List α
+
+  namespace Word
+    notation:max w "⟦" a ".." b "⟧" => List.extract w a b
+    notation:max w "⟦" a "..*⟧" => List.drop a w
+
+    variable {α: Type u} (w: Word α)
+
+    def range: Set ℤ := { i: ℤ | i ≥ 0 ∧ i < w.length }
+
+    instance (i: ℤ): Decidable (i ∈ w.range) := by
+      unfold range
+      infer_instance
+
+    def get' (i: ℤ) (h: i ∈ w.range) := w.get ⟨
+      i.toNat,
+      by simp only [range, ge_iff_le, Set.mem_setOf_eq] at h; omega
+    ⟩
+
+    def get'? (i: ℤ): Option α :=
+      if h: i ∈ w.range
+      then some (w.get' i h)
+      else none
+  end Word
+
+
+end Word
+
+
+
+section LanguageDefinitions -- MARK: LanguageDefinitions
+
+  class DefinesLanguage (CA) (α: outParam (Type)) where
+    L: CA -> Language α
+
+
+  variable {CA: Type*} [Alphabet α]
+
+  def ℒ [d: DefinesLanguage CA α] (s: (Set CA)): Set (Language α) :=
+      fun L => ∃ ca: CA, ca ∈ s ∧ L = DefinesLanguage.L ca
+
+
+end LanguageDefinitions
+
+
+
+section CellAutomaton -- MARK: CellAutomaton
+
+  structure CellAutomaton where
+    Q: Type
+    [alphabetQ: Alphabet Q]
+    δ: Q → Q → Q → Q
+
+  attribute [instance] CellAutomaton.alphabetQ
+
+
+  def Config (Q: Type*) := ℤ → Q
+
+  variable (C: CellAutomaton)
+
+  namespace CellAutomaton
+
+    def next (c: Config C.Q): Config C.Q :=
+      fun p => C.δ (c (p - 1)) (c p) (c (p + 1))
+
+    def nextt: Config C.Q → ℕ → Config C.Q := apply_iterated C.next
+
+
+    /-- A set is quiescent if every element stays the same when it is just surrounded by other elements from the set. -/
+    def quiescent_set (Q: Set C.Q) := ∀ (a b c: Q), C.δ a b c = b
+
+    /-- A state is quiescent if it stays the same when it is just surrounded by itself. -/
+    def quiescent (q: C.Q) := C.quiescent_set { q }
+
+    /-- A set state is closed if no matter what, cells having such a state remain in that set. -/
+    def delta_closed_set (Q: Set C.Q) := ∀ a (b: Q) c, C.δ a b c ∈ Q
+    /-- A state is dead if no matter what, it doesn't change. -/
+    def dead (q: C.Q) := C.delta_closed_set {q}
+
+    def left_independent := ∀ (q1 q2 q3 q1'), C.δ q1 q2 q3 = C.δ q1' q2 q3
+    def right_independent := ∀ (q1 q2 q3 q3'), C.δ q1 q2 q3 = C.δ q1 q2 q3'
+
+    /-- A state is initial if it cannot be created -/
+    def initial (q: C.Q) := ∀ a b c, C.δ a b c = q → b = q
+
+  end CellAutomaton
+
+
+  def δδ { C: CellAutomaton } (q: C.Q) := C.δ q q q
+
+  def δδt { C: CellAutomaton } (q: C.Q) := apply_iterated δδ q
+
+end CellAutomaton
+
+
+
+section LCellAutomaton -- MARK: LCellAutomaton
+
+  /--
+  A cellular automaton that can map words to a configuration.
+  This is the basis for cellular automata that can recognize languages.
+  -/
+  structure LCellAutomaton (α: Type) extends CellAutomaton where
+    embed: α → Q
+    border: Q
+
+  namespace LCellAutomaton
+
+    variable [Alphabet α] (C: LCellAutomaton α)
+
+    def embed_word (w: Word α): Config C.Q :=
+      fun p =>
+        if h: p ∈ w.range
+        then C.embed (w.get' p h)
+        else C.border
+
+    /-- To compute the nth configuration of a word, we compute the nth follow configuration of the word's embedding. -/
+    def comp (w: Word α) := C.nextt (C.embed_word w)
+
+
+    def scan_temporal (t: ℕ) (p: ℤ) (w: Word α): Word C.Q :=
+      List.map (C.comp w · p) (List.range t)
+
+    def scan_temporal_rt (w: Word α): Word C.Q :=
+      C.scan_temporal w.length 0 w
+
+    /-- A state is an internal state if embedding an input does not produce it. -/
+    def internal_state (q: C.Q) := ∀ a: α, C.embed a ≠ q
+
+
+  end LCellAutomaton
+
+end LCellAutomaton
+
+
+
+section tCellAutomaton -- MARK: tCellAutomaton
+
+  structure tCellAutomaton (α: Type) extends LCellAutomaton α where
+    t: ℕ → ℕ
+    p: ℕ → ℕ
+    F_pos: Q → Bool
+
+  def tCellAutomaton.L (C: tCellAutomaton α): Language α := fun w =>
+    (C.comp w (C.t w.length)) 0 |> C.F_pos
+
+  def tCellAutomatons (α: Type): Set (tCellAutomaton α) := Set.univ
+
+  instance : DefinesLanguage (tCellAutomaton α) α where
+    L ca := ca.L
+
+
+  def tCellAutomaton.similar [Alphabet α] (C1 C2: tCellAutomaton α): Prop := C1.L = C2.L ∧ C1.t = C2.t ∧ C1.p = C2.p
+
+  section
+
+    variable (α: Type)
+
+    def t_rt (S: Set (tCellAutomaton α)) := { C ∈ S | ∀ n, C.t n = n - 1 }
+    def t_2n (S: Set (tCellAutomaton α)) := { C ∈ S | ∀ n, C.t n = 2 * n }
+    def t_lt (S: Set (tCellAutomaton α)) := { C ∈ S | ∃ c: ℕ, ∀ n, C.t n = c * n }
+
+    def CA   := { C ∈ tCellAutomatons α | C.p = fun _ => 0 }
+    def CA_rt := CA α |> t_rt α
+    def CA_2n := CA α |> t_2n α
+    def CA_lt := CA α |> t_lt α
+
+    def CAr  := { C ∈ tCellAutomatons α | C.p = fun n => n }
+
+    def OCA  := { C ∈ CA α | C.left_independent }
+    def OCA_rt := OCA α |> t_rt α
+    def OCA_2n := OCA α |> t_2n α
+    def OCA_lt := OCA α |> t_lt α
+
+    def OCAr  := { C ∈ CAr α | C.right_independent }
+    def OCAr_rt := OCAr α |> t_rt α
+    def OCAr_2n := OCAr α |> t_2n α
+    def OCAr_lt := OCAr α |> t_lt α
+
+  end
+
+end tCellAutomaton
+
+
+
+instance (C: tCellAutomaton α) (w: Word α) : Decidable (w ∈ C.L) := by
+  unfold tCellAutomaton.L
+  unfold Membership.mem
+  unfold Language.instMembershipList
+  simp [Set.Mem]
+  infer_instance
+
+
+instance (C: tCellAutomaton α) : DecidablePred C.L :=
+  fun w => by
+    unfold tCellAutomaton.L
+    infer_instance
+
+
+
+section tCellAutomatonWithAdvice -- MARK: tCellAutomatonWithAdvice
+
+  structure Advice (α: Type) (Γ: Type) where
+    f: Word α → Word Γ
+    len: ∀ w: Word α, (f w).length = w.length
+
+  @[simp]
+  lemma advice_len {α Γ} (adv: Advice α Γ) (w: Word α): (adv.f w).length = w.length := by
+    simp [adv.len]
+
+  def zip_words {α β} (w: List α) (a: List β) := List.zipWith (·,·) w a
+
+  infixl:65 " ⊗ " => zip_words
+
+  @[app_unexpander zip_words]
+  def unexpand_zip_words : Lean.PrettyPrinter.Unexpander
+  | `($_ $w $a) => `($w ⊗ $a)
+  | _ => throw ()
+
+
+  namespace Advice
+    section
+      variable {Γ: Type} {adv: Advice α Γ}
+
+      def annotate (w: Word α): Word (α × Γ) := w ⊗ (adv.f w)
+
+      def prefix_stable: Prop :=
+        ∀ w: Word α, ∀ i: ℕ,
+          adv.f (w.take i) = (adv.f w).take i
+    end
+
+    def compose {Γ₁: Type} {Γ₂: Type} (adv1: Advice α Γ₁) (adv2: Advice Γ₁ Γ₂): Advice α Γ₂ :=
+      ⟨ fun w => adv2.f (adv1.f w), by simp [adv1.len, adv2.len] ⟩
+
+  end Advice
+
+
+  structure tCellAutomatonWithAdvice (α: Type) where
+    Γ: Type
+    [alphabetΓ: Alphabet Γ]
+    adv: Advice α Γ
+    C: tCellAutomaton (α × Γ)
+
+  attribute [instance] tCellAutomatonWithAdvice.alphabetΓ
+
+  def tCellAutomatonWithAdvice.L (C: tCellAutomatonWithAdvice α): Language α := { w | C.C.L (C.adv.annotate w) }
+
+
+  def tCellAutomatonWithAdvice.with_advice {Γ: Type} [Alphabet Γ] (S: Set (tCellAutomaton (α × Γ))) (adv: Advice α Γ)
+      : Set (tCellAutomatonWithAdvice α) :=
+    { tCellAutomatonWithAdvice.mk Γ adv C | C ∈ S }
+
+  instance {Γ: Type} [Alphabet Γ] : HAdd (Set (tCellAutomaton (α × Γ))) (Advice α Γ) (Set (tCellAutomatonWithAdvice α)) where
+    hAdd S adv := tCellAutomatonWithAdvice.with_advice S adv
+
+  instance [Alphabet α] : DefinesLanguage (tCellAutomatonWithAdvice α) α where
+    L ca := tCellAutomatonWithAdvice.L ca
+
+
+
+
+  def Advice.rt_closed {Γ: Type} [Alphabet α] [Alphabet Γ] (f: Advice α Γ) :=
+      ℒ (CA_rt (α × Γ) + f) = ℒ (CA_rt α)
+
+
+
+
+
+  structure FiniteStateTransducer (α: Type) (β: Type) where
+      Q: Type
+      [alphabetQ: Alphabet Q]
+      δ: Q → α → Q
+      q0: Q
+      f: Q → β
+
+  namespace FiniteStateTransducer
+    attribute [instance] FiniteStateTransducer.alphabetQ
+
+    section
+      variable (M: FiniteStateTransducer α β)
+
+      def δ?: M.Q → Option α → M.Q
+        | q, none => q
+        | q, some a => M.δ q a
+
+      def scanr_step a
+      | (q, w) => (M.δ q a, M.f (M.δ q a) :: w)
+
+      def scanr_q (q: M.Q) (w: Word α): Word β :=
+        (w.foldr (M.scanr_step) (q, [])).snd
+
+      def scanr w := M.scanr_q M.q0 w
+
+      def scanr_reduce_q (q: M.Q): Word α → M.Q
+      | []   => q
+      | c::cs => M.δ (scanr_reduce_q q cs) c
+
+      def scanr_reduce := M.scanr_reduce_q M.q0
+
+      def map_input (f: γ → α): FiniteStateTransducer γ β := {
+        Q := M.Q
+        δ := fun q a => M.δ q (f a)
+        q0 := M.q0
+        f := M.f
+      }
+
+      @[simp, grind =]
+      lemma scanr_q_len (q: M.Q) (w: List α):
+        (M.scanr_q q w).length = w.length := by
+        unfold scanr_q
+        induction w with
+        | nil => simp []
+        | cons a ws ih => simp [scanr_step, ih]
+
+
+      @[simp, grind =]
+      lemma scanr_len (w: List α): (M.scanr w).length = w.length := by
+        simp [scanr, scanr_q_len]
+    end
+
+  end FiniteStateTransducer
+
+
+  def FiniteStateTransducer.advice [Alphabet α] [Alphabet β] (M: FiniteStateTransducer α β): Advice α β :=
+    ⟨
+      fun w => M.scanr w,
+      by grind [FiniteStateTransducer.scanr_len]
+    ⟩
+
+
+
+
+
+  structure CArtTransducer (α: Type) (Γ: Type) [Alphabet α] [Alphabet Γ] extends LCellAutomaton α where
+    f: Q → Γ
+
+
+  def CArtTransducer.advice [Alphabet α] [Alphabet Γ] (adv: CArtTransducer α Γ): Advice α Γ :=
+    ⟨
+      fun w => (adv.scan_temporal_rt w).map adv.f,
+      by grind [LCellAutomaton.scan_temporal_rt, LCellAutomaton.scan_temporal]
+    ⟩
+
+
+
+
+
+
+  structure TwoStageAdvice (α: Type) (Γ: Type) [Alphabet α] [Alphabet Γ]  where
+    β: Type
+    [alphabetβ: Alphabet β]
+    C: CArtTransducer α β
+    M: FiniteStateTransducer β Γ
+
+  attribute [instance] TwoStageAdvice.alphabetβ
+
+  namespace TwoStageAdvice
+    variable {α: Type} {Γ: Type} [Alphabet α] [Alphabet Γ] {adv: TwoStageAdvice α Γ}
+
+    def advice: Advice α Γ :=
+      ⟨
+        adv.M.advice.f ∘ adv.C.advice.f,
+        by grind [Advice.len]
+      ⟩
+
+  end TwoStageAdvice
+
+
+
+  def Advice.is_two_stage_advice [Alphabet α] [Alphabet Γ] (adv: Advice α Γ): Prop :=
+    ∃ ts_adv: TwoStageAdvice α Γ, adv = ts_adv.advice
+
+
+
+
+
+  def Advice.prefixes_in_L (L: Language α) [h: DecidablePred L]: Advice α Bool :=
+    ⟨
+      fun w => (List.range w.length).map (fun i => decide (L (w⟦0..i+1⟧))),
+      by simp
+    ⟩
+
+
+  def Advice.exp: Advice α Bool :=
+    ⟨
+      fun w => (List.range w.length).map fun i => i == 2 ^ (Nat.log2 i),
+      by simp
+    ⟩
+
+
+
+  def Advice.from_len_marker (f: ℕ → Option ℕ): Advice α Bool :=
+    ⟨
+      fun w =>
+        let idx := f w.length
+        (List.range w.length).map fun i => some (i + 1) == idx,
+      by simp
+    ⟩
+
+
+
+  def middle_idx (n: ℕ) := n / 2
+
+  def Advice.middle (α): Advice α Bool := Advice.from_len_marker (some ∘ middle_idx)
+
+  #guard (List.range 10).map (fun n => (n, middle_idx n)) =
+    [(0,0), (1,0), (2,1), (3,1), (4,2), (5,2), (6,3), (7,3), (8,4), (9,4)]
+
+  #guard (@Advice.middle Unit).f (List.replicate 10 ()) =
+    [false, false, false, false, true, false, false, false, false, false]
+
+
+
+  -- runs the biggest value 2^k such that 2^(k+1) <= n, if such exists
+  def exp_middle_idx (n: ℕ) :=
+    (List.range n).map (2 ^ ·)
+    |> List.filter (· * 2 ≤ n)
+    |> List.max?
+
+  -- Marks the biggest exponent of 2 that is less than or equal to the length of the word
+  def Advice.exp_middle (α): Advice α Bool := Advice.from_len_marker exp_middle_idx
+
+  #guard (List.range 10).map (fun n => (n, exp_middle_idx n)) =
+    [(0, none), (1, none), (2, some 1), (3, some 1), (4, some 2), (5, some 2), (6, some 2), (7, some 2), (8, some 4), (9, some 4)]
+
+  #guard (@Advice.exp_middle Unit).f (List.replicate 10 ()) =
+    [false, false, false, true, false, false, false, false, false, false]
+
+
+
+  def Advice.shift_left_advice {adv: Advice α Γ} (extension: Word α): Advice α Γ :=
+    ⟨
+      fun w => (adv.f (w.append extension)).drop extension.length,
+      by simp [adv.len]
+    ⟩
+
+end tCellAutomatonWithAdvice
