CellularAutomatas_old/proofs/cart_transducers.lean
@@ -1,0 +1,609 @@
+import CellularAutomatas.defs
+import Mathlib.Data.List.Basic
+import Mathlib.Data.Nat.Basic
+import Mathlib.Data.Nat.Find
+import Mathlib.Data.Int.Cast.Basic
+import Mathlib.Data.Fintype.Option
+import Mathlib.Tactic.Ring
+
+namespace CellularAutomatas
+
+private lemma list_map_congr {α β} {f g : α → β} {l : List α} (h : ∀ x ∈ l, f x = g x) : l.map f = l.map g := by
+  induction l with
+  | nil => rfl
+  | cons a l ih =>
+  simp only [List.map_cons, List.cons.injEq]
+  constructor
+  · apply h; simp
+  · apply ih; intro x hx; apply h; simp [hx]
+
+
+lemma nextt_congr (C: CellAutomaton) (c1 c2: Config C.Q) (t: ℕ) (i: ℤ):
+    (∀ j, i - t ≤ j ∧ j ≤ i + t → c1 j = c2 j) →
+    (C.nextt c1 t) i = (C.nextt c2 t) i := by
+  induction t generalizing i c1 c2 with
+  | zero =>
+    intro h
+    simp [CellAutomaton.nextt, apply_iterated]
+    apply h
+    constructor <;> omega
+  | succ t ih =>
+    intro h
+    simp [CellAutomaton.nextt, apply_iterated]
+    -- The goal is now nextt (next c1) t i = nextt (next c2) t i
+    apply ih
+    intro j hj
+    unfold CellAutomaton.next
+    congr 1
+    · apply h
+      constructor <;> omega
+    · apply h
+      constructor <;> omega
+    · apply h
+      constructor <;> omega
+
+theorem LCellAutomaton.scan_temporal_independence [Alphabet α] (C: LCellAutomaton α) (p s: Word α):
+  (C.scan_temporal_rt (p ++ s)).take p.length = C.scan_temporal_rt p := by
+  unfold LCellAutomaton.scan_temporal_rt LCellAutomaton.scan_temporal
+  rw [← List.map_take, List.take_range, min_eq_left (by simp)]
+  apply list_map_congr
+  intro t ht
+  rw [List.mem_range] at ht
+  apply nextt_congr
+  intro j hj
+  unfold LCellAutomaton.embed_word
+  split_ifs with h1 h2
+  · congr 1
+    unfold Word.get'
+    simp only [List.get_eq_getElem]
+    apply List.getElem_append_left
+  · exfalso; unfold Word.range at *; simp at *; omega
+  · exfalso; unfold Word.range at *; simp at *; omega
+  · rfl
+
+theorem CArtTransducer.scan_temporal_independence [Alphabet α] [Alphabet Γ] (C: CArtTransducer α Γ) (p s: Word α):
+  (C.advice.f (p ++ s)).take p.length = C.advice.f p := by
+  unfold CArtTransducer.advice
+  simp
+  rw [←List.map_take]
+  rw [LCellAutomaton.scan_temporal_independence]
+
+
+
+
+
+
+section id
+
+  def ca_id (α : Type) [Alphabet α] : CArtTransducer α α := {
+    Q := α
+    δ := fun _ _ r => r
+    embed := id
+    border := default
+    f := id
+  }
+
+  lemma ca_id_comp_p0 {α : Type} [Alphabet α] {w : Word α} (h: t < w.length):
+    (ca_id α).comp w t 0 = w[t] := by
+    unfold LCellAutomaton.comp
+
+    have shift_next c : (ca_id α).next c = fun i => c (i + 1) := by
+      funext i
+      simp [CellAutomaton.next, ca_id]
+
+    have shift_nextt k c i: ((ca_id α).nextt c k) i = c (i + k) := by
+      induction k generalizing c with
+      | zero =>
+        simp [CellAutomaton.nextt, apply_iterated]
+      | succ k ih =>
+        rw [CellAutomaton.nextt, apply_iterated]
+        simp only [Nat.iterate]
+        rw [shift_next]
+        rw [← apply_iterated]
+        rw [← CellAutomaton.nextt]
+        rw [ih]
+        simp
+        ring_nf
+
+    rw [shift_nextt]
+    unfold LCellAutomaton.embed_word
+    dsimp [ca_id]
+    unfold Word.get'
+    unfold Word.range
+    grind
+
+  @[simp]
+  lemma ca_id_scan_temporal [Alphabet α]: (ca_id α).advice.f = id := by
+    funext w
+    rw [id_eq]
+    apply List.ext_getElem
+    · simp
+    · intro i h_i h_len
+      unfold CArtTransducer.advice LCellAutomaton.scan_temporal_rt LCellAutomaton.scan_temporal
+      conv in (ca_id α).f => change id
+      simp [ca_id_comp_p0 h_len]
+
+end id
+
+
+
+
+
+
+
+
+def word_dvd_k_ext (k: ℕ) (w_len: ℕ) := (w_len - (w_len % w_len)) % w_len
+
+def word_dvd_k (k: ℕ) (w: Word α): Word (Option α) :=
+  w.map (fun a => some a) ++ List.replicate (word_dvd_k_ext k w.length) none
+
+def L_dvd_k (k: ℕ) (L: Language α): Language (Option α) := { word_dvd_k k w | w ∈ L }
+
+theorem L_in_RT_iff_L_dvd_k_in_RT (k: ℕ) (L: Language α):
+    L ∈ ℒ (CA_rt α) ↔ (L_dvd_k k L) ∈ ℒ (CA_rt (Option α)) := by
+  sorry
+
+
+notation x "³"  => Fin 3 → x
+
+
+
+
+
+def triple_at {Q} (c: ℕ → Q) (i: ℕ): Q³ := fun o => c (i + o)
+
+
+def CArtTransducer.compo [Alphabet α] [Alphabet β] {C: CArtTransducer α β} (w: Word α) (t: ℕ): Config β := C.f ∘ (C.toLCellAutomaton.comp w t)
+
+def CArtTransducer.comport [Alphabet α] [Alphabet β] {C: CArtTransducer α β} (w: Word α): Word β :=
+  (List.range w.length).map (fun t => C.compo w t 0)
+
+def CArtTransducer.compio [Alphabet α] [Alphabet β] {C: CArtTransducer α β} (c: Config α) (t: ℕ): Config β := C.f ∘ (C.toLCellAutomaton.nextt (C.embed ∘ c) t)
+
+
+
+structure CompressToDiag where
+  {α: Type}
+  {β: Type}
+  [_inst_α: Alphabet α]
+  [_inst_β: Alphabet β]
+  C_orig: CArtTransducer α β
+
+attribute [instance] CompressToDiag._inst_α
+attribute [instance] CompressToDiag._inst_β
+
+namespace CompressToDiag
+
+  variable (e: CompressToDiag)
+
+  def C: CArtTransducer e.α (Option (e.β³)) := sorry
+
+  theorem spec (w: Word e.α) (t: ℕ) (p: ℤ):
+      e.C.compo w t p =
+        if p >= 0 ∧ t = 2 * p + 3
+        then some (triple_at (e.C_orig.compo w · 0) (3 * p).natAbs)
+        else none
+        := by
+    sorry
+
+end CompressToDiag
+
+
+
+
+
+
+
+structure CompressToΛ where
+  {α: Type}
+  {β: Type}
+  [_inst_α: Alphabet α]
+  [_inst_β: Alphabet β]
+  C_orig: CArtTransducer α β
+  border: β
+
+attribute [instance] CompressToΛ._inst_α
+attribute [instance] CompressToΛ._inst_β
+
+namespace CompressToΛ
+  variable (e: CompressToΛ)
+
+  def C: CArtTransducer e.α (Option (e.β³)) := sorry
+
+  def decode_cfg (w: Word e.α): Config (e.β³) :=
+    fun p =>
+      if p ≥ 0
+      then triple_at (e.C_orig.compo w . 0) (3 * p).natAbs
+      else (fun _ => e.border)
+
+  theorem spec (w: Word e.α) (t: ℕ) (p: ℤ):
+      e.C.compo w t p =
+        if t = 3 + 2 * p.natAbs
+        then some (e.decode_cfg w p)
+        else none
+        := by
+    sorry
+
+end CompressToΛ
+
+lemma intCastEq {k: ℕ} [NeZero k] (p: ℤ): (Fin.intCast p: Fin k) = (p % k) := by
+  sorry
+
+
+
+structure SpeedupKx where
+  k: ℕ
+  [inst: NeZero k]
+  C_orig: CellAutomaton
+
+attribute [instance] SpeedupKx.inst
+
+namespace SpeedupKx
+  section
+    variable {Q: Type}
+    variable (k: ℕ) [NeZero k]
+
+    def compress (c: Config Q): Config (Fin k → Q) :=
+      fun p => fun j => c (p * k + j)
+
+    def decompress (c: Config (Fin k → Q)): Config Q :=
+      fun p => c (p / k) (Fin.intCast p)
+
+    lemma compress_decompress (c: Config Q):
+      decompress k (compress k c) = c := by
+        funext p
+        unfold decompress compress
+        congr
+        rw [intCastEq]
+        rw [Int.emod_def]
+        grind only
+  end
+
+  variable (e: SpeedupKx)
+
+  def Q' := Fin e.k → e.C_orig.Q
+
+  def local_config (a b c: e.Q'): Config e.C_orig.Q :=
+      fun p => if p <= -e.k then a (Fin.intCast 0) else
+        if p < 0 then a (Fin.intCast (p + e.k))
+        else if p < e.k then b (Fin.intCast p)
+        else c (Fin.intCast (p - e.k))
+
+  def to_local_config (c: Config (e.C_orig.Q)): e.Q' := fun j => c j
+
+  def C: CellAutomaton := {
+    Q := Fin e.k → e.C_orig.Q
+    δ := fun a b c =>
+      e.to_local_config (e.C_orig.nextt (e.local_config a b c) e.k)
+  }
+
+
+  lemma compression_k_step (c: Config e.C_orig.Q):
+      e.C.next (compress e.k c) = compress e.k (e.C_orig.nextt c e.k) :=
+        sorry
+
+  theorem spec (c: Config e.C_orig.Q):
+      ∀ t, e.C.nextt (compress e.k c) t = compress e.k (e.C_orig.nextt c (e.k * t)) :=
+        sorry
+
+end SpeedupKx
+
+
+
+structure SimFromΛ where
+  {α: Type}
+  {β: Type}
+  {γ: Type}
+  [_inst_α: Alphabet α]
+  [_inst_β: Alphabet β]
+  [_inst_γ: Alphabet γ]
+  C_ctl: CArtTransducer α (Option β)
+  C_inr: CArtTransducer β γ
+
+attribute [instance] SimFromΛ._inst_α
+attribute [instance] SimFromΛ._inst_β
+attribute [instance] SimFromΛ._inst_γ
+
+namespace SimFromΛ
+  variable (e: SimFromΛ)
+
+  structure Q1 where
+    state: e.C_ctl.Q
+    counter: Fin 3
+  deriving Inhabited, DecidableEq, Fintype
+
+
+  def C: CArtTransducer e.α (Option e.γ) := {
+    Q := Option (Q1 e × e.C_inr.Q)
+    δ := fun a b c =>
+      match (a, b, c) with
+      | (some qa, some (qb, _), some qc) =>
+        if qb.counter = 2
+        then sorry
+        else none
+      | _ => none
+    border := default
+    embed := sorry
+    f := sorry
+  }
+
+  variable (c_ctl: Config e.α)
+  variable (c_inr: Config e.β)
+
+  def c_ctl_computes_c_inr: Prop :=
+    ∀ (t: ℕ) (p: ℤ),
+    e.C_ctl.compio c_ctl t p =
+      if t = 3 + 2 * p.natAbs
+      then some (c_inr p)
+      else none
+
+
+  theorem spec (h_CM: e.c_ctl_computes_c_inr c_ctl c_inr) (t: ℕ) (p: ℤ):
+    e.C.compio c_ctl (3 + 3 * t) 0 = some (e.C_inr.compio c_inr t 0) := by
+      sorry
+end SimFromΛ
+
+
+structure DecompressTriple where
+  {α: Type}
+  {β: Type}
+  [_inst_α: Alphabet α]
+  [_inst_β: Alphabet β]
+  C_orig: CArtTransducer α (Option (β³))
+
+attribute [instance] DecompressTriple._inst_α
+attribute [instance] DecompressTriple._inst_β
+
+namespace DecompressTriple
+
+  variable (e: DecompressTriple)
+
+  def C (e: DecompressTriple): CArtTransducer e.α (Option e.β) := sorry
+
+
+  theorem spec (c: Config e.α) (t: ℕ) (v: (e.β³))
+    (h: ∀ o: Fin 3, e.C_orig.compio c (t + o) 0 = if o == 0 then some v else none):
+      ∀ o: Fin 3, (e.C.compio c (t + o) 0) = some (v o) := by
+    sorry
+
+
+  def h_cond (c: Config e.α) (k: ℕ): Prop :=
+      ∀ (t: ℕ), ((e.C_orig.compio c (t + k) 0)).isSome == ((t - k) % 3 == 0)
+
+  theorem spec2 (c: Config e.α) (h: e.h_cond c k) (t: ℕ):
+        e.C.compio c t 0 =
+          if t < k then none
+          else (e.C_orig.compio c ((t - k) / 3 * 3) 0).map (. (Fin.ofNat 3 (t - k)))
+      := by
+    sorry
+
+end DecompressTriple
+
+
+
+
+structure SpeedupKSteps where
+  {α: Type}
+  {β: Type}
+  [inst1: Alphabet α]
+  [inst2: Alphabet β]
+  C_orig: CArtTransducer α β
+  k: ℕ
+
+attribute [instance] SpeedupKSteps.inst1
+attribute [instance] SpeedupKSteps.inst2
+
+namespace SpeedupKSteps
+
+  variable (e: SpeedupKSteps)
+
+  def C: CArtTransducer e.α e.β := sorry
+
+  theorem spec: e.C.compo w w.length = e.C_orig.compo w (w.length + e.k) := sorry
+
+end SpeedupKSteps
+
+
+
+
+
+def triple_to_fun (v: α × α × α): α³ :=
+    fun
+      | 0 => v.1
+      | 1 => v.2.1
+      | 2 => v.2.2
+
+
+/-
+  def C_ctl {e: Composition} : LCellAutomaton e.α := sorry
+  def f : e.C_ctl.Q → Option (e.C2.Q³) := sorry
+
+
+  variable (w: Word e.α)
+  def c_orig: Config (e.C2.Q³) := SpeedupKx.compress 3 (e.C2.embed_word (e.C1.advice.f w))
+
+  lemma C_ctl_spec: e.f (e.C_ctl.comp w t p) =
+      if t = 3 + 2 * p.natAbs then some (e.c_orig w p)
+      else none := by
+    sorry
+-/
+
+
+def CArtTransducer.map_out [Alphabet α] [Alphabet β] [Alphabet γ] (C: CArtTransducer α β) (f: β → γ):
+    CArtTransducer α γ := {
+  Q := C.Q
+  δ := C.δ
+  embed := C.embed
+  border := sorry
+  f := f ∘ C.f
+}
+
+structure Composition where
+  α: Type
+  β: Type
+  γ: Type
+  [_inst_α: Alphabet α]
+  [_inst_β: Alphabet β]
+  [_inst_γ: Alphabet γ]
+  C2: CArtTransducer β γ
+  C1: CArtTransducer α β
+
+attribute [instance] Composition._inst_α
+attribute [instance] Composition._inst_β
+attribute [instance] Composition._inst_γ
+
+def LCellAutomaton.embed_c [Alphabet α] [Alphabet β] {C: LCellAutomaton α} (c: Option α): C.Q :=
+  match c with
+  | none => C.border
+  | some x => C.embed x
+
+
+structure CellAutomatonT (α β: Type) where
+  Q: Type
+  [alphabetQ: Alphabet Q]
+  δ: Q → Q → Q → Q
+  embed: α → Q
+  project: Q → β
+
+def CellAutomatonT.embed_config {α β: Type} (C: CellAutomatonT α β) (c: Config α): Config C.Q :=
+  fun p => C.embed (c p)
+
+def CellAutomatonT.project_config {α β: Type} (C: CellAutomatonT α β) (c: Config C.Q): Config β :=
+  fun p => C.project (c p)
+
+def CellAutomatonT.comp {α β: Type} (C: CellAutomatonT α β) (c: Config α) (t: ℕ): Config β :=
+  C.project_config (C.nextt (C.embed_config c) t)
+
+
+--@[coe]
+def Word.toConfig {α : Type} (w : Word α) : Config (Option α) := w.get'?
+--instance : CoeOut (Word α) (Config (Option α)) := ⟨Word.toConfig⟩
+
+def Word.toConfig2 {α : Type} (w : Word α) : Config (Option α) := w.get'?
+instance {C: CellAutomatonT (Option α) β} : Coe (Word α) (Config C.Q) := ⟨C.embed_config ∘ Word.toConfig2⟩
+
+
+abbrev CellAutomaton2 (α: Type) := CellAutomatonT (Option α) Bool
+
+def foo (e: CellAutomaton2 α) (w: Word α) := e.nextt w
+#print foo
+
+namespace Composition
+  variable (e: Composition)
+
+  -- α -> (Option C2.Q³)
+  def C1_Λ: CompressToΛ := {
+    α := e.α
+    β := e.C2.Q
+    -- α -> C2.Q
+    C_orig := e.C1.map_out (fun v => e.C2.embed v)
+    border := e.C2.border
+  }
+/-
+
+We want to show:
+C.trace_rt = C2.trace_rt ∘ C1.trace_rt
+<=>
+C.trace_rt w = C2.trace_rt (C1.trace_rt w)
+
+
+
+
+
+
+
+-/
+
+
+  -- LCellAutomaton α := CellAutomaton (Option α) Bool
+
+
+  -- C.trace [w] = C2.trace [C1.trace [w]]
+
+  -- restrict_border: * * # = #, # # # = #
+  -- VC1.comp_extract [w] = compress3 [C1.trace [w]]
+  -- then (Sim VC1 (C2_3x)).nextt [w] (3t + 3) 0 = C2_3x.nextt (compress3 [C1.trace [w]]) t 0
+  --   = (C2.nextt [C1.trace [w]]) 3t 0
+
+
+  -- c_ctl := compress [w]: (Config C1.Q)
+  -- c_inr := compress [C1_Λ.comport w]: (Option ³)
+  -- lemma l1: C1_Λ.c_ctl_computes_c_inr c_ctl c_inr
+  -- lemma l2:
+  -- C2.Q³ -> C2.Q³
+  def C2_3x: SpeedupKx := {
+    k := 3
+    C_orig := e.C2.toCellAutomaton
+  }
+
+  def C_sim: SimFromΛ := {
+    α := e.α
+    β := e.C2.Q³
+    γ := e.γ³
+    C_ctl := e.C1_Λ.C -- α -> (Option C2.Q³)
+    C_inr := {
+      toCellAutomaton := e.C2_3x.C
+      border := default
+      embed := id
+      f := fun q => fun o => e.C2.f (q o)
+    }
+  }
+
+  --
+  def C_decomp: DecompressTriple := {
+    α := e.α
+    β := e.γ
+    C_orig := e.C_sim.C
+  }
+
+  def C_exact: SpeedupKSteps := {
+    α := e.α
+    β := e.γ
+    C_orig := e.C_decomp.C.map_out (fun o => o.getD default)
+    k := 3
+  }
+
+  def C: CArtTransducer e.α e.γ := e.C_exact.C
+
+  theorem spec: e.C.comport = e.C2.comport ∘ e.C1.comport := by
+    sorry
+
+
+end Composition
+
+/-
+
+* Lc(adv2) is rt+adv1
+* Lc(adv2 o adv1) is rt
+* adv2 o adv1 is rt-closed
+
+
+
+* put input + advice on the diagonal (3-tupel)
+* then run the simulation on the 3x speedup automaton
+* we have now the results for (3t, 3t+1, 3t+2) at 3t+3 (from step 3) (or something like this)
+  * we need to smear it out , so that 3t+k is available at 3t + k + 3, for k = 0,1,2
+  * then we speed it up by 3 steps
+  * if temporal_trace[i] is w[i], then temporal_trace[i - 1] must be w[i - 1],
+  * because it cannot see the end
+
+-/
+
+
+
+
+def CArtTransducer.rt_closed [Alphabet α] [Alphabet β] [Alphabet γ] (t: CArtTransducer β γ): t.advice.rt_closed :=
+  sorry
+
+
+
+
+def CArtTransducer.compose [Alphabet α] [Alphabet β] [Alphabet γ] (t1: CArtTransducer β γ) (t2: CArtTransducer α β):
+    CArtTransducer α γ :=
+  sorry
+
+def CArtTransducer.compose_spec [Alphabet α] [Alphabet β] [Alphabet γ]
+    {t1: CArtTransducer β γ} {t2: CArtTransducer α β}:
+    (CArtTransducer.compose t1 t2).advice.f =
+      t1.advice.f ∘ t2.advice.f := by
+        sorry
