CellularAutomatas_old/proofs/is_two_stage_of_rt_closed_and_prefix_stable.lean
@@ -1,0 +1,415 @@
+import Mathlib.Data.Set.Basic
+import Mathlib.Data.Nat.Basic
+import Mathlib.Data.Nat.Find
+import Mathlib.Data.Fintype.Basic
+import Mathlib.Data.Fintype.Pi
+import Mathlib.Data.Fintype.Option
+import Mathlib.Computability.Language
+import Mathlib.Data.Set.Lattice
+import Mathlib.Data.Nat.Lattice
+import Mathlib.Data.Fintype.Prod
+import Mathlib.Tactic.Ring
+import Mathlib.Tactic.Linarith
+import Mathlib.Logic.Function.Iterate
+import Mathlib.Data.List.Basic
+import CellularAutomatas.defs
+import CellularAutomatas.proofs.cart_transducers
+import CellularAutomatas.proofs.finite_state_transducers
+
+namespace CellularAutomatas
+
+--def extend_word_to k: Word α → Word (Option α)
+/-
+def Lk L k := sorry
+
+
+lemma X (Ls1 Ls2: Set (Language α))
+  (h1: P Ls1) (h2: P Ls2)
+  (h: ∀ L ∈ ℒ CA_rt, ∃ L2 ∈ Ls2, (∀ w ∈ L, w.length.div k) → w ∈ L2):
+    ∀ α, Ls1 α ⊆ Ls2 α := sorry
+
+Let L ∈ Ls1.
+
+-/
+
+
+@[simp]
+lemma adv_empty (adv : Advice α Γ) : adv.f [] = [] := by
+  have h_len : (adv.f []).length = 0 := by simp [adv.len]
+  rw [List.length_eq_zero_iff.mp h_len]
+
+
+
+lemma tCellAutomatonWithAdvice.elem_L_iff {O: tCellAutomatonWithAdvice α}:
+  w ∈ O.L ↔ (O.adv.annotate w) ∈ O.C.L := by rfl
+
+lemma tCellAutomaton.elem_L_iff {C: tCellAutomaton α}:
+  w ∈ C.L ↔ C.F_pos ((C.comp w (C.t w.length)) 0) := by rfl
+
+@[simp]
+lemma scan_temporal_length {C: LCellAutomaton α} (w : Word α) :
+  (C.scan_temporal_rt w).length = w.length := by
+  unfold LCellAutomaton.scan_temporal_rt LCellAutomaton.scan_temporal
+  simp
+
+
+lemma scan_temporal_in_F_pos {C: tCellAutomaton α} (hC: C ∈ CA_rt α) {w: Word α} (i: Nat) (h: i < (C.scan_temporal_rt w).length ):
+    C.F_pos (C.scan_temporal_rt w)[i] = true ↔ w.take (i+1) ∈ C.L := by
+  rw [scan_temporal_length] at h
+  have h_len : i < w.length := h
+  have h_take_len : (w.take (i+1)).length = i + 1 := by
+    rw [List.length_take]
+    rw [min_eq_left]
+    omega
+  have h_t : C.t (w.take (i+1)).length = i := by
+    simp [CA_rt, t_rt] at hC
+    rw [hC.2]
+    rw [h_take_len]
+    simp
+  dsimp [tCellAutomaton.L, Membership.mem, Set.Mem]
+  rw [h_t]
+  unfold LCellAutomaton.scan_temporal_rt LCellAutomaton.scan_temporal
+  rw [List.getElem_map]
+  simp
+  congr 1
+  apply nextt_congr
+  intro j hj
+  unfold LCellAutomaton.embed_word
+  split_ifs with h1 h2
+  · -- j in range of w and w.take
+    unfold Word.get'
+    simp
+  · -- j in range of w but not w.take
+    unfold Word.range at *
+    simp at *
+    grind
+  · -- j not in range of w but in range of w.take
+    unfold Word.range at *
+    simp at *
+    grind
+  · -- neither
+    rfl
+
+def ProdCA (α: Type) (β: Type) [DecidableEq β] [Fintype β] (f: β → LCellAutomaton α): LCellAutomaton α := {
+  Q := ∀ b: β, (f b).Q
+  δ := fun qL qC qR a => (f a).δ (qL a) (qC a) (qR a)
+  embed := fun a b => (f b).embed a
+  border := fun b => (f b).border
+}
+
+namespace ProdCA
+
+
+variable {β: Type} [Alphabet β]
+variable {f: β → LCellAutomaton α}
+
+lemma comp (f: β → LCellAutomaton α)
+    (w: Word α) (t: ℕ) (i: ℤ):
+    (ProdCA α β f).comp w t i = fun b => (f b).comp w t i := by
+  unfold LCellAutomaton.comp
+  unfold CellAutomaton.nextt
+
+  have nextt_proj (c: Config (ProdCA α β f).Q) (t: ℕ) (i: ℤ) (b: β):
+      (ProdCA α β f).next^[t] c i b = (f b).next^[t] (fun j => c j b) i := by
+    induction t generalizing i c with
+    | zero => rfl
+    | succ t ih =>
+      rw [Function.iterate_succ]
+      rw [Function.iterate_succ]
+      dsimp
+      rw [ih]
+      dsimp [CellAutomaton.next, ProdCA]
+      rfl
+
+  funext b
+  simp [apply_iterated]
+  rw [nextt_proj]
+  apply congr_arg (fun c => (f b).next^[t] c i)
+  funext j
+  unfold LCellAutomaton.embed_word
+  dsimp [ProdCA]
+  split_ifs <;> rfl
+
+
+-- zipMany over { x => [a, b, c], y => [1, 2, 3] } should be  [ {x => a, y => 1}, {x => b, y => 2}, {x => c, y => 3} ]
+
+def zipMany {γ: β -> Type v} [∀ b, Inhabited (γ b)] (f: (b: β) → Word (γ b)) : Word ((b: β) -> (γ b)) :=
+  let n := (f default).length
+  (List.range n).map fun i => fun b => (f b).getD i default
+
+lemma zipMany_get? {γ: β -> Type v} [∀ b, Inhabited (γ b)] (f: (b: β) → Word (γ b)) (i: ℕ):
+    (ProdCA.zipMany f)[i]? = if i < (f default).length then some (fun b => (f b).getD i default) else none := by
+  simp [zipMany]
+  grind
+
+lemma scan_temporal (f: β → LCellAutomaton α) (w: Word α):
+    (ProdCA α β f).scan_temporal t p w = zipMany (fun b => (f b).scan_temporal t p w) := by
+  unfold LCellAutomaton.scan_temporal
+  simp [zipMany]
+  intro t ht
+  funext b
+  rw [comp]
+  grind
+
+end ProdCA
+
+open Classical
+
+
+attribute [ext] Advice
+
+variable {α: Type} [Alphabet α]
+variable {Γ: Type} [Alphabet Γ]
+
+def L_c (adv: Advice α Γ) (c: Γ) : Language α :=
+  { w | (adv.f w).getLast? = some c }
+
+namespace LcInRt
+
+def DiagonalShiftCA (A : Type) [Alphabet A] : LCellAutomaton A := {
+  Q := Option A
+  δ := fun _ _ r => r
+  embed := some
+  border := none
+}
+
+@[simp]
+lemma DiagonalShiftCA_comp_p0  (w : Word α) :
+  (DiagonalShiftCA α).comp w t 0 = w[t]? := by
+  unfold LCellAutomaton.comp
+
+  have shift_next c : (DiagonalShiftCA α).next c = fun i => c (i + 1) := by
+    funext i
+    simp [CellAutomaton.next, DiagonalShiftCA]
+
+  have shift_nextt k c i: ((DiagonalShiftCA α).nextt c k) i = c (i + k) := by
+    induction k generalizing c with
+    | zero =>
+      simp [CellAutomaton.nextt, apply_iterated]
+    | succ k ih =>
+      rw [CellAutomaton.nextt, apply_iterated]
+      simp only [Nat.iterate]
+      rw [shift_next]
+      rw [← apply_iterated]
+      rw [← CellAutomaton.nextt]
+      rw [ih]
+      simp
+      ring_nf
+
+  rw [shift_nextt]
+  unfold LCellAutomaton.embed_word
+  dsimp [DiagonalShiftCA]
+  unfold Word.get'
+  unfold Word.range
+  grind
+
+lemma DiagonalShiftCA_scan_temporal {Q : Type} [Alphabet Q] (w : Word Q) :
+  (DiagonalShiftCA Q).scan_temporal_rt w = w.map some := by
+  unfold LCellAutomaton.scan_temporal_rt LCellAutomaton.scan_temporal
+  apply List.ext_getElem
+  · simp
+  · intro i h_i h_len
+    simp [←getElem?_pos]
+
+
+def AdvCALc (c : Γ) : tCellAutomaton (α × Γ) := {
+  toLCellAutomaton := DiagonalShiftCA (α × Γ)
+  t := fun n => n - 1
+  p := fun _ => 0
+  F_pos := fun q => match q with
+    | some (_, g) => g == c
+    | none => false
+}
+
+lemma myCA_in_rt (c : Γ) : AdvCALc c ∈ CA_rt (α × Γ) := by
+  simp [CA_rt, t_rt, AdvCALc, tCellAutomatons, CA]
+
+lemma scan_temporal_get_last {C: tCellAutomaton α} (w : Word α):
+  (C.scan_temporal_rt w).getLast? = if w = [] then none else ((C.comp w (w.length - 1)) 0) := by
+  cases h_w : w.length with
+  | zero =>
+    simp [LCellAutomaton.scan_temporal_rt, LCellAutomaton.scan_temporal]
+    have h_nil : w = [] := List.length_eq_zero_iff.mp h_w
+    subst h_nil
+    unfold LCellAutomaton.comp
+    unfold LCellAutomaton.embed_word
+    simp
+  | succ n =>
+    have h_len_pos : w.length > 0 := by rw [h_w]; simp
+    have h_scan_len : (C.scan_temporal_rt w).length = w.length := scan_temporal_length w
+    have h_scan_pos : (C.scan_temporal_rt w).length > 0 := by rw [h_scan_len]; exact h_len_pos
+
+    rw [List.getLast?_eq_some_getLast (List.ne_nil_of_length_pos h_scan_pos)]
+    simp
+    rw [List.getLast_eq_getElem]
+    unfold LCellAutomaton.scan_temporal_rt LCellAutomaton.scan_temporal
+    simp
+    grind
+
+
+def O (adv : Advice α Γ) (c : Γ) : tCellAutomatonWithAdvice α := ⟨Γ, adv, AdvCALc c⟩
+
+
+lemma O_L_eq_L_c (adv : Advice α Γ) (c : Γ) : (O adv c).L = L_c adv c := by
+  ext w
+  simp [tCellAutomatonWithAdvice.L, L_c]
+  let w_ann := adv.annotate w
+  have h_len : w_ann.length = w.length := by
+    simp [w_ann, Advice.annotate, zip_words, adv.len]
+
+  change (AdvCALc c).F_pos ((AdvCALc c).comp w_ann ((AdvCALc c).t w_ann.length) 0) ↔ (adv.f w).getLast? = some c
+  dsimp [AdvCALc]
+  rw [DiagonalShiftCA_comp_p0]
+
+  cases h_w : w.length with
+  | zero =>
+    have h_nil : w = [] := List.length_eq_zero_iff.mp h_w
+    subst h_nil
+    have h_ann_nil : w_ann = [] := by simp [w_ann, Advice.annotate, zip_words]
+    rw [h_ann_nil]
+    simp
+  | succ n =>
+    have h_ann_len_pos : w_ann.length > 0 := by rw [h_len, h_w]; simp
+    have h_idx : w_ann.length - 1 < w_ann.length := by omega
+
+    rw [List.getElem?_eq_getElem (h:=h_idx)]
+    simp
+
+    have h_idx_f : (adv.f w).length - 1 < (adv.f w).length := by
+      rw [adv.len]
+      rw [h_len] at h_idx
+      exact h_idx
+
+    have h_snd : (w_ann[w_ann.length - 1]).2 = (adv.f w)[(adv.f w).length - 1] := by
+      simp [w_ann, Advice.annotate, zip_words]
+
+    rw [h_snd]
+
+    have h_f_ne : adv.f w ≠ [] := by
+      rw [← List.length_pos_iff_ne_nil]
+      rw [adv.len, h_w]
+      simp
+
+    rw [List.getLast?_eq_some_getLast h_f_ne]
+    rw [List.getLast_eq_getElem]
+    simp
+
+
+end LcInRt
+
+lemma L_c_in_rt (adv: Advice α Γ) (h: adv.rt_closed) (c: Γ) :
+      ∃ M : tCellAutomaton α, M ∈ CA_rt α ∧ M.L = L_c adv c := by
+  let O := LcInRt.O adv c
+  have h_in : O.L ∈ ℒ (CA_rt (α × Γ) + adv) := by
+    use O
+    constructor
+    · change O ∈ tCellAutomatonWithAdvice.with_advice (CA_rt (α × Γ)) adv
+      simp [tCellAutomatonWithAdvice.with_advice]
+      use LcInRt.AdvCALc c
+      exact ⟨LcInRt.myCA_in_rt c, rfl⟩
+    · rfl
+
+  erw [h] at h_in
+  rcases h_in with ⟨M, hM_in, hM_L⟩
+  use M
+  constructor
+  · exact hM_in
+  · change DefinesLanguage.L M = L_c adv c
+    rw [← hM_L, LcInRt.O_L_eq_L_c]
+
+noncomputable def CALc (adv: Advice α Γ) (h: adv.rt_closed) (c: Γ) : tCellAutomaton α :=
+  Classical.choose (L_c_in_rt adv h c)
+
+lemma CALc_spec_1 (adv: Advice α Γ) (h: adv.rt_closed) (c: Γ) :
+    (CALc adv h c) ∈ CA_rt α :=
+  (Classical.choose_spec (L_c_in_rt adv h c)).1
+
+lemma CALc_spec_2 (adv: Advice α Γ) (h: adv.rt_closed) (c: Γ) :
+    (CALc adv h c).L = L_c adv c :=
+  (Classical.choose_spec (L_c_in_rt adv h c)).2
+
+
+
+namespace PrefixStableProof
+
+  variable (adv: Advice α Γ) (h1: adv.rt_closed)
+
+  noncomputable abbrev M_prod := ProdCA α Γ (fun c => (CALc adv h1 c).toLCellAutomaton)
+
+  noncomputable def t_map (q: (M_prod adv h1).Q) : Γ :=
+    let valid_c := Finset.univ.filter (fun c => (CALc adv h1 c).F_pos (q c))
+    valid_c.toList.head?.getD default
+
+
+
+  noncomputable def ts_adv : TwoStageAdvice α Γ := {
+    C := ⟨ M_prod adv h1, t_map adv h1 ⟩
+    β := Γ
+    M := FiniteStateTransducer.M_id Γ
+  }
+
+  lemma getLastOfTake (h: i < w.length): (List.take (i + 1) w).getLast? = w[i]? := by
+    grind
+
+  lemma f (h2: adv.prefix_stable): (ts_adv adv h1).advice = adv := by
+    apply Advice.ext
+    funext w
+    simp [TwoStageAdvice.advice]
+    unfold ts_adv
+    simp
+
+    unfold CArtTransducer.advice
+    simp [LCellAutomaton.scan_temporal_rt]
+    rw [ProdCA.scan_temporal]
+    conv =>
+      pattern LCellAutomaton.scan_temporal _ _ _ _
+      rw [←LCellAutomaton.scan_temporal_rt]
+
+    apply List.ext_getElem?
+
+    intro i
+    rw [List.getElem?_map]
+    erw [ProdCA.zipMany_get?]
+    simp
+
+    by_cases h_i : i < w.length
+    case neg => simp [h_i]
+
+    unfold t_map
+    simp
+
+
+    simp [scan_temporal_in_F_pos (CALc_spec_1 adv h1 _), h_i]
+    simp [CALc_spec_2 adv h1]
+    unfold L_c
+
+    have h2 := h2 w (i+1)
+
+    -- TODO@lean: This is annoying
+    suffices
+      some ((Finset.univ.filter (fun c => List.getLast? (adv.f (List.take (i + 1) w)) = some c)).toList.head?.getD default) = (adv.f w)[i]? by
+        grind
+
+    rw [h2]
+    have : i < (adv.f w).length := by
+      simp [h_i, adv.len]
+
+    rw [getLastOfTake this]
+
+    rw [List.getElem?_eq_getElem this]
+    simp
+    have h_singleton : (Finset.univ.filter (fun c => (adv.f w)[i] = c)) = {(adv.f w)[i]} := by grind
+    rw [h_singleton]
+    simp
+
+
+end PrefixStableProof
+
+
+
+theorem is_two_stage_of_rt_closed_and_prefix_stable (adv: Advice α Γ) (h1: adv.rt_closed) (h2: adv.prefix_stable):
+    adv.is_two_stage_advice := by
+
+    unfold Advice.is_two_stage_advice
+    use PrefixStableProof.ts_adv adv h1
+    simp [PrefixStableProof.f adv h1 h2]
